restructure directory

src/proposer.dfy
@@ -1,57 +1,97 @@
 module Proposer {
-	class Proposer<T(==)>
+	class SingleProposer<T(==)>
 	{
 		var majority:  int; // half of assumed active acceptors
-		var round:     int; // current and largest encountered round from acceptors
-		var prepared:  seq<int>; // set of answered prepares
-		// previously  set<int>;
+		var round:     int; // our current round
 		var value:     T; // own value or value of acceptor with largest round
+		var largest:   int; // largest encountered round from acceptors
+		var prepared:  set<int>; // set of answered prepares
+		// previously  set<int>; changed due to bug with Length operator
+
+		ghost var acceptors: map<int, T>; // a map<round, value> of prepared acceptors
 
 		constructor (rnd: int, val: T)
-		modifies this;
+			modifies this;
+			ensures value == val;
+			ensures valid();
 		{
-			majority := 0;
-			round    := rnd;
-			value    := val;
+			majority  := 0;
+			round     := rnd;
+			value     := val;
+			largest   := -1;
+			acceptors := map[];
 		}
 
 		method Promise(id: int, acp_round: int, acp_value: T)
-			returns (largest: int, val: T)
-			requires true;
+			returns (ok: bool, large: int, val: T)
+			requires valid();
+			// acceptors with equal round have equal value
+			requires (acp_round == largest ==> acp_value == value)
+				&& (acp_round in acceptors ==> acceptors[acp_round] == acp_value);
 			modifies this;
-			ensures round >= acp_round;
+			ensures  valid();
+			ensures  id in prepared && large == round >= largest >= acp_round;
+			// acceptors with equal round have equal value
+			ensures  (acp_round == largest ==> acp_value == value)
+				&& (acp_round in acceptors ==> acceptors[acp_round] == acp_value);
+			// majority implies no accepted round is > largest encountered
+			ensures  ok ==> (forall rnd :: rnd in acceptors ==> (
+				rnd <= largest
+			));
 		{
 			// log response from acceptor
-			prepared := prepared + [id];
-			// previously  prepared := prepared + {id};
-			// were there any prior proposals?
-			if round < acp_round {
-				value := acp_value;
-				round := acp_round;
+			prepared  := prepared + {id};
+			acceptors := acceptors[acp_round := acp_value]; // update ghost
+
+			// Any prior accepted proposals? adopt round and value
+			if largest < acp_round {
+				largest := acp_round;
+				value   := acp_value;
 			}
-			assert round >= acp_round;
-			largest, val := Evaluate_majority();
-			return largest, val;
+			// due to round in sent prepare messages, pick the highest round
+			if round < largest { round := largest; }
+
+			ok := Evaluate_majority();
+			return ok, round, value;
 		}
 
-		method Evaluate_majority() returns (rnd: int, val: T)
+		method Evaluate_majority() returns (ok: bool)
 		{
 			// got required majority of acceptors?
 			if |prepared| >= majority {
 				// TODO: store state
-				return round, value;
+				return true;
 			}
-			// else return nothing? 0, 0? 0, null?
+			return false;
 		}
 
-		method Configure(num_acceptors: int)
-			returns (rnd: int, val: T)
+		method Reconfigure(num_acceptors: int)
+			returns (ok: bool, rnd: int, val: T)
+			requires valid();
 			modifies this;
+			ensures valid();
 		{
 			majority := num_acceptors/2 + 1;
-			// re-evaluate |prepared| because we might not get more promises!
-			rnd, val := Evaluate_majority();
-			return rnd, val;
+			// re-evaluate |prepared| because we might NOT get more promises!
+			ok := Evaluate_majority();
+			// due to round in sent prepare messages, pick the highest round
+			if round < largest { return ok, largest, value; }
+			else { return ok, round, value; }
+		}
+
+		method SetMajority(maj: int)
+			requires valid();
+			modifies this;
+			ensures  valid();
+		{ majority := maj; }
+
+		predicate valid()
+			reads this;
+		{
+			// no promised acceptor's round is larger than ours
+			(forall rnd :: rnd in acceptors ==> rnd <= round)
+			// acceptors with equal round have equal value
+			&& (largest in acceptors ==> acceptors[largest] == value)
 		}
 	}
 }
