src/proposer_old.dfy
@@ -1,0 +1,57 @@
+module Proposer {
+	class Proposer<T(==)>
+	{
+		var majority:  int; // half of assumed active acceptors
+		var round:     int; // current and largest encountered round from acceptors
+		var prepared:  seq<int>; // set of answered prepares
+		// previously  set<int>;
+		var value:     T; // own value or value of acceptor with largest round
+
+		constructor (rnd: int, val: T)
+		modifies this;
+		{
+			majority := 0;
+			round    := rnd;
+			value    := val;
+		}
+
+		method Promise(id: int, acp_round: int, acp_value: T)
+			returns (largest: int, val: T)
+			requires true;
+			modifies this;
+			ensures round >= acp_round;
+		{
+			// log response from acceptor
+			prepared := prepared + [id];
+			// previously  prepared := prepared + {id};
+			// were there any prior proposals?
+			if round < acp_round {
+				value := acp_value;
+				round := acp_round;
+			}
+			assert round >= acp_round;
+			largest, val := Evaluate_majority();
+			return largest, val;
+		}
+
+		method Evaluate_majority() returns (rnd: int, val: T)
+		{
+			// got required majority of acceptors?
+			if |prepared| >= majority {
+				// TODO: store state
+				return round, value;
+			}
+			// else return nothing? 0, 0? 0, null?
+		}
+
+		method Configure(num_acceptors: int)
+			returns (rnd: int, val: T)
+			modifies this;
+		{
+			majority := num_acceptors/2 + 1;
+			// re-evaluate |prepared| because we might not get more promises!
+			rnd, val := Evaluate_majority();
+			return rnd, val;
+		}
+	}
+}
