src/v0.2/acceptor.dfy
@@ -1,0 +1,70 @@
+class Acceptor<T(==)>
+{
+  var promise:  int;
+  var accepted: Accepted<T>;
+
+  constructor (value: T)
+    modifies this;
+    ensures valid();
+  {
+    promise  := -1;
+    accepted := new Accepted(value);
+  }
+
+  method Prepare(round: int, value: T) returns (ok: bool, acp: Accepted<T>)
+    requires valid();
+    modifies this;
+  ensures valid() && promise >= round;
+  {
+    acp := accepted;
+    ok  := false;
+    // is the round at least as new as our promise
+    // and we have not already accepted it?
+    if round >= promise && round != accepted.round {
+      promise := round;
+      assert promise > accepted.round;
+      // TODO: store state?
+      ok := true;
+    }
+  }
+
+  method Accept(round: int, value: T) returns (ok: bool, acp: Accepted<T>)
+    requires valid();
+    modifies this, accepted;
+  ensures valid() && promise >= round;
+  {
+    acp := accepted;
+    ok  := false;
+    // is the round at least as new as our promise?
+    if round >= promise {
+      promise         := round;
+      accepted.round  := round;
+      accepted.value  := value;
+      // TODO: store state
+      ok := true;
+    }
+  }
+
+  method Get() returns (rnd: int, acp: int, val: T)
+    requires valid();
+  {
+    rnd := promise;
+    acp := accepted.round;
+    val := accepted.value;
+  }
+
+  predicate valid()
+    reads this, accepted;
+  { accepted != null && promise >= accepted.round }
+}
+
+class Accepted<T(==)>
+{
+  var round: int;
+  var value: T;
+
+  constructor (val: T)
+    modifies this;
+    ensures round == -1; // yes, this has to be explicitly stated!
+  { round := -1; value := val; }
+}
