src/v0.2/learner.dfy
@@ -1,0 +1,49 @@
+class Learner<T(==)>
+{
+  var majority: int; // half of assumed active acceptors
+  var current:  int; // the highest encountered round number
+  var accepted: map<T, seq<int>>; // accepted values mapping sets of acceptors that share it
+  // previously map<T, set<int>>;
+
+  constructor ()
+    modifies this;
+  {
+    majority := 0;
+    current  := -1;
+  }
+
+  method Learn(id: int, round: int, value: T) returns (learned: bool, ret: T)
+    modifies this;
+  {
+    // is the acceptor up to date?
+    if round > current {
+      current := round;
+      accepted := map[]; // new boys in town. out with the old
+    }
+    if round == current {
+      // add acceptor to set
+      if value !in accepted {
+        // this is the first occurrance of value
+        // accepted[value] := {id}
+        accepted := accepted[ value := [id] ];
+      } else {
+        // value already has a set. update with old set union {id}
+        // accepted[value] += {id}
+        accepted := accepted[ value := accepted[value] + [id] ];
+      }
+      // do we have a majority?
+      if |accepted[value]| >= majority {
+        // yay
+        return true, value;
+      }
+    }
+    return false, value;
+  }
+
+  method Configure(num_acceptors: int)
+    modifies this;
+  {
+    majority := num_acceptors/2 + 1;
+    // re-evaluate?
+  }
+}
